# 3진법 뒤집기

```JAVA
import java.util.ArrayList;
class Solution {
    public int solution(int n) {
        int answer = 0;

        int length = (int)(Math.log10(n)+1);

        ArrayList<Integer> n3Arr = new ArrayList<>();
        int i=0;
        while (n >= 3) {
            int n3 = n%3;
            n3Arr.add(n3);
            n = n/3;
            i++;
        }
        n3Arr.add(n);

        int n3Length = n3Arr.size();
        int[] reverseN3Arr = new int[n3Length];
        for(int j=0; j<n3Length; j++) {
            reverseN3Arr[j] = n3Arr.get(j);
        }

        int n10 = 0;
        for(int j=0; j<n3Length; j++) {
            n10 = reverseN3Arr[n3Length - (j+1)] * (int)Math.round(Math.pow(3, j));
            answer += n10;
        }
        
		return answer;
    }
}
```

[프로그래머스] https://programmers.co.kr/learn/courses/30/lessons/68935
